# Derivatives in the video

## Derivatives

- How much does output change for small changes in input

e = a\*b \
d = e + c \
L = d*f

## Derivatie 'L' w.r.t "d" and "f"**

${\normalsize L = d*f}$ \
\
Hence: &nbsp; ${\normalsize {\partial L \over \partial d }= f}$ &nbsp; &nbsp; &nbsp; &nbsp; ${\normalsize {\partial L \over \partial f } = d}$

## Derivatie 'd' w.r.t "c" and "e"**

${\normalsize d = c+e}$ \
\
Hence: &nbsp; ${\normalsize {\partial d \over \partial c } = 1}$ &nbsp; &nbsp; &nbsp; &nbsp; ${\normalsize {\partial d \over \partial e } = 1}$

**Chain rule:** ${\normalsize {\partial L \over \partial c } = {\partial L \over \partial d } * {\partial d \over \partial c }}$
